user 3, session 6414, part 9

diffs-annotated/3/user-3-session-6414.v
@@ -19,11 +19,24 @@ SearchPattern _.
 Remove Search Blacklist "Raw" "Proofs".
 Unset Search Output Name Only.
 Timeout 1 Print LoadPath.
-Print Abstraction.
-Print LayerAbstraction.
+Module Log (d: OneDiskAPI)<: LogAPI.
+Definition init : proc InitResult.
+Admitted.
+Definition get : proc (list block).
+Admitted.
+Definition append : list block -> proc bool.
+Admitted.
+Definition reset : proc unit.
+Admitted.
+Definition recover : proc unit.
+Admitted.
 Definition abstr : Abstraction State := {| abstraction := fun _ _ => True |}.
-Redirect "/var/folders/5x/1mdbpbjd7012l971fq0zkj2w0000gn/T/coqznJnVn"
-Print Ltac Signatures.
+Theorem init_ok : init_abstraction init recover abstr inited_any.
+Proof.
+Admitted.
+Theorem get_ok : proc_spec get_spec get recover abstr.
+Proof.
+Admitted.
 Theorem append_ok :
   forall v, proc_spec (append_spec v) (append v) recover abstr.
 Proof.
@@ -34,22 +47,4 @@ Admitted.
 Theorem recover_wipe : rec_wipe recover abstr no_wipe.
 Proof.
 Admitted.
-Redirect "/var/folders/5x/1mdbpbjd7012l971fq0zkj2w0000gn/T/coqDeDx9w"
-Print Ltac Signatures.
-Timeout 1 Print Grammar tactic.
-Add Search Blacklist "Raw" "Proofs".
-Set Search Output Name Only.
-Redirect "/var/folders/5x/1mdbpbjd7012l971fq0zkj2w0000gn/T/coqnAF75v"
-SearchPattern _.
-Remove Search Blacklist "Raw" "Proofs".
-Unset Search Output Name Only.
 End Log.
-Redirect "/var/folders/5x/1mdbpbjd7012l971fq0zkj2w0000gn/T/coqofeRUT"
-Print Ltac Signatures.
-Timeout 1 Print Grammar tactic.
-Add Search Blacklist "Raw" "Proofs".
-Set Search Output Name Only.
-Redirect "/var/folders/5x/1mdbpbjd7012l971fq0zkj2w0000gn/T/coqxssI6y"
-SearchPattern _.
-Remove Search Blacklist "Raw" "Proofs".
-Unset Search Output Name Only.
